haskell/adi/Test/Debug.hs
@@ -4,12 +4,11 @@ module  Test.Debug
     )   where
 
 import DSL
-import Macro
 import Interpret
 
 main :: IO ()
 main = do
-   evalIO e3
+   evalIO e2
 
 e1 :: Expr
 e1 = eLam "x" (eVar "x") 
@@ -18,8 +17,8 @@ e2 :: Expr
 e2 = eApp (eLam "x" (eLam "y" (eVar "x"))) (eNum 4)
 
 e3 :: Expr 
-e3 = eApp (eFac "f" "n") (eNum 5)
+e3 = eApp eFac (eNum 5)
 
 e4 :: Expr
-e4 = eDiv (eNum 0) (eNum 1)
+e4 = eApp2 eDiv (eNum 0) (eNum 1)
 
