haskell/aop/Poly.hs
@@ -1,0 +1,49 @@
+{-# LANGUAGE LambdaCase             #-}
+
+module  Poly
+    (   Poly    (..)
+    ,   main
+    )   where
+
+import Test.Hspec
+import Test.QuickCheck
+import Data.Bifunctor
+import Data.Functor.Foldable
+
+newtype Poly a = Poly { unPoly :: [a] } 
+
+main :: IO ()
+main = hspec $ describe "Testing equivalence of implementations" $ do
+    spec01
+
+spec01 :: Spec
+spec01 = it "Checked eval0 ~ eval1" $ do
+    property prop01
+
+prop01 :: [Integer] -> Integer -> Bool
+prop01 xs x = eval0 (Poly xs) x == eval1 (Poly xs) x 
+
+pow :: (Num a) => a -> Integer -> a
+pow x n
+    | n < 0     = error "pow: negative argument"
+    | n == 0    = 1
+    | otherwise = x * pow x (n - 1)
+
+-- initial type of bifunctor ListF
+mu :: ListF a [a] -> [a]
+mu = \case
+    Nil         -> []
+    Cons x xs   -> x : xs
+
+triangle_ :: (a -> a) -> ListF a [a] -> [a]
+triangle_ f = mu . bimap id (map f) 
+
+triangle :: (a -> a) -> [a] -> [a]
+triangle = cata . triangle_
+
+eval0 :: (Num a) => Poly a -> a -> a
+eval0 p x = sum $ map (\(a,n) -> a * pow x n) $ zip (unPoly p) [0..]
+
+eval1 :: (Num a) => Poly a -> a -> a
+eval1 p x = sum $ triangle (*x) $ unPoly p 
+
