coq/cttwc/doubleNeg.v
@@ -54,3 +54,74 @@ Proof.
       apply H4, H1, H3.
     - intros H3. apply H1. intros H4. apply H2, H4, H3.
 Qed.
+
+
+Lemma L7 : forall (X Y:Prop), (~X -> ~Y) <-> (Y -> ~~X).
+Proof.
+    intros X Y. split; intros H1 H2 H3; apply H1; assumption.
+Qed.
+
+Lemma L8 : forall (X Y:Prop), (X -> Y) -> ~~(~X \/ Y).
+Proof.
+    intros X Y H1 H2. 
+    assert (~Y) as H3. { intros H3. apply H2. right. assumption. }
+    assert (~~X) as H4. {intros H4. apply H2. left. assumption. }
+    assert (~X) as H5. { intros H5. apply H3, H1. assumption. }
+    apply H4. assumption.
+Qed.
+
+
+Lemma L9 : forall (a:Type) (p:a -> Prop), 
+    ~(forall (x:a), ~p x) <-> ~~ exists (x:a), p x.
+Proof.
+    intros a p. split; intros H1 H2; apply H1.
+    - intros x H3. apply H2. exists x. assumption.
+    - intros [x H3]. apply (H2 x). assumption.
+Qed.
+
+Lemma L10 : forall (X Y:Prop), ~~X \/ ~~Y -> ~~(X \/ Y).
+Proof.
+    intros X Y [H1|H1] H2; apply H1; intros H3; apply H2.
+    - left. assumption.
+    - right. assumption.
+Qed.
+
+Lemma L11 : forall (a:Type) (p:a -> Prop), 
+    (exists (x:a), ~~ p x) -> ~~ exists (x:a), p x.
+Proof.
+    intros a p [x H1] H2. apply H1. intros H3. apply H2. exists x. assumption.
+Qed.
+
+Lemma L12 : forall (a:Type) (p:a -> Prop), 
+    ~~(forall (x:a), p x) -> forall (x:a), ~~ p x.
+Proof.
+    intros a p H1 x H2. apply H1. intros H3. apply H2, H3.
+Qed.
+
+(* Coq meta-property not provable in Coq: The double negation of a quantifier   *)
+(* free proposition which is provable using LEM, is provable.                   *)
+
+(* X \/ ~X is provable using LEM, hence ...                                     *)
+Lemma L13 : forall (X:Prop), ~~(X \/ ~X).
+Proof.
+    intros X H1.
+    assert (~X) as H2.  { intros H2. apply H1. left.  assumption. }
+    assert (~~X) as H3. { intros H3. apply H1. right. assumption. }
+    apply H3. assumption.
+Qed.
+
+(* ~~X -> X is provable using LEM, hence...                                     *)
+Lemma L14 : forall (X:Prop), ~~(~~X -> X).
+Proof.
+    intros X H1. apply H1. intros H2. exfalso. apply H2. intros H3. apply H1.
+    intros H4. assumption.
+Qed.
+
+Lemma L15 : forall (X Y:Prop), ~~(~(X /\ Y) -> ~X \/ ~Y).
+Proof.
+    intros X Y H1. apply H1. intros H2. 
+    assert (~~X) as H3. { intros H3. apply H1. intros H4. left.  assumption. }
+    assert (~~Y) as H4. { intros H4. apply H1. intros H5. right. assumption. }
+    exfalso. apply H3. intros H5. apply H4. intro H6. apply H2. 
+    split; assumption.
+Qed.
