coq/logic/Nil.v
@@ -1,0 +1,15 @@
+Require Import List.
+Require Import In.
+
+Lemma nil_charac : forall (v:Type) (xs:list v),
+    xs = nil <-> forall (x:v), ~ (x::xs). 
+Proof.
+    intros v xs. split; intros H1.
+    - intros x H2. destruct xs as [|x' xs].
+        + inversion H2.
+        + inversion H1.
+    - destruct xs as [|x' xs].
+        + reflexivity.
+        + exfalso. apply (H1 x'). left. reflexivity.
+Qed.
+
