coq/set/Lang1/Apply.v
@@ -1,18 +1,40 @@
 Require Import Utils.Replace.
+Require Import Utils.Composition.
 
+Require Import Core.Set.
+
+Require Import Lang1.Valid.
 Require Import Lang1.Syntax.
+Require Import Lang1.Semantics.
+Require Import Lang1.Environment.
+Require Import Lang1.Substitution.
 
-(* A formula with a free variable could be viewed as a predicate. Viewed as a   *)
-(* predicate a formula may need to be 'evaluated' at another variable, and this *)
-(* evaluation corresponds to a variable substitution. In the following, we      *)
-(* formalize this evaluation by substituting the variable '0' by the argument n *)
-(* This choice of variable '0' is arbitrary, but having this default choice     *)
-(* leads to simpler syntax as there is no need to spell out which variable is   *)
-(* being substituted. There is nothing deep here, as we are just creating a new *)
-(* formula from an old one. The ability to apply a formula viewed as predicate  *)
-(* to variables in particularly important for two variables as this is needed   *)
-(* to express the axiom schema of replacement.                                  *)
+(* A formula with a free variable could be viewed as a predicate which needs to *)
+(* be 'evaluated' at some variable, where such evaluation corresponds to a      *)
+(* variable substitution. In the following, we formalize this evaluation by     *)
+(* substituting the variable '0' by the argument 'n'. This choice of variable   *)
+(* '0' is arbitrary, but having this default choice leads to simpler syntax as  *)
+(* there is no need to spell out which variable is being replaced. There is     *)
+(* nothing deep here, as we are just creating a new formula from an old one.    *)
+(* The ability to apply a formula viewed as predicate to variables is important *)
+(* for two variables, and is needed to express the axiom schema of replacement. *)
 
 Definition apply (p:Formula) (n:nat) : Formula := fmap (replace 0 n) p.
 
 Notation "p $ n" := (apply p n) (at level 60, right associativity) : set_scope.
+
+Open Scope set_scope.
+
+(* Semantics of (p $ n) in an environement where n is bound to set x is the     *)
+(* same as the semantics of p in an environment where 0 is bound to x. However, *)
+(* we cannot hope to obtain this semantics equivalence without assuming that    *)
+(* the replacement of variable 0 by n is a valid substitution for p.            *)
+
+(*
+Lemma evalApply1 : forall (e:Env) (p:Formula) (n:nat) (x:set),
+    Valid (replace 0 n) p ->
+        eval1 e (p $ n) n x <-> eval1 e p 0 x.
+Proof.
+    unfold eval1, apply. intros e p n x H. rewrite Substitution.
+Show.
+*)
