lean/while/BExp.lean
@@ -2,3 +2,4 @@ import Env
 
 -- Shallow embedding for boolean expressions
 def BExp : Type := Env -> Prop
+
