lean/while/Reduction.lean
@@ -2,17 +2,21 @@ import Stmt
 
 open Stmt
 
+axiom LEM : forall (p:Prop), p ∨ ¬p
+
 -- Small step semantics, aka reduction relation
 inductive Reduce : Stmt → Env → Stmt → Env → Prop
 | ASN     : ∀ (x:string) (a:AExp) (s:Env), Reduce (assign x a) s skip (bindVar x a s)
 | SEQ_STEP: ∀ (e₁ e₁' e₂:Stmt) (s s':Env),
     Reduce e₁ s e₁' s' →
-    Reduce (e₁ ;; e₂) s (skip ;; e₂) s'
+    Reduce (e₁ ;; e₂) s (e₁' ;; e₂) s'
 | SEQ_SKIP: ∀ (e:Stmt) (s:Env), Reduce (skip ;; e) s e s
 | IF_T    : ∀ (b:BExp) (e₁ e₂:Stmt) (s:Env), b s → Reduce (ite b e₁ e₂) s e₁ s
 | IF_F    : ∀ (b:BExp) (e₁ e₂:Stmt) (s:Env), ¬ b s → Reduce (ite b e₁ e₂) s e₂ s
 | WHILE   : ∀ (b:BExp) (e:Stmt) (s:Env),
     Reduce (while b e) s (ite b (e ;; (while b e)) skip) s
+
+open Reduce
 
 -- Predicate expressing that no further reduction is possible
 def Value (e:Stmt) (s:Env) : Prop := ¬ (∃ (e':Stmt) (s':Env), Reduce e s e' s')
@@ -21,13 +25,17 @@ def Value (e:Stmt) (s:Env) : Prop := ¬ (∃ (e':Stmt) (s':Env), Reduce e s e' s
 lemma seq_reduce : ∀ (e₁ e₂:Stmt) (s:Env),
   (∃ (e':Stmt) (s':Env), Reduce (e₁ ;; e₂) s e' s') :=
 begin
-  intros e₁, cases e₁ with x a; intros e₂ s,
-    {existsi e₂, existsi s, constructor},
-    {},
-    {},
-    {},
-    {},
-    {},
+  intros e₁, induction e₁ with x a e₁ e₁' IH1 IH1' b e₁ e₁' IH1 IH1' b e₁ IH1;
+  intros e₂ s,
+    { existsi e₂, existsi s, constructor },
+    { existsi (skip ;; e₂), existsi (bindVar x a s), apply SEQ_STEP, apply ASN },
+    { clear IH1', cases (IH1 e₁' s) with e H1, cases H1 with s' H1,
+      existsi (e ;; e₂), existsi s', apply SEQ_STEP, assumption },
+    { cases (LEM (b s)) with H1 H1,
+      { existsi (e₁ ;; e₂), existsi s, apply SEQ_STEP, apply IF_T, assumption },
+      { existsi (e₁' ;; e₂), existsi s, apply SEQ_STEP, apply IF_F, assumption }},
+    { existsi ((ite b (e₁ ;; while b e₁) skip) ;; e₂), existsi s,
+      apply SEQ_STEP, apply WHILE},
 end
 
 lemma Value_is_skip : ∀ (e:Stmt) (s:Env), Value e s ↔ e = skip :=
